Hs/HsJudgment.lean
@@ -1,0 +1,199 @@
+import Hs.HsTerm
+import SystemFD.Ctx
+import SystemFD.Substitution
+import SystemFD.Judgment
+
+def HsValidHeadVariable (t : HsTerm) (test : Nat -> Bool) : Prop :=
+  ∃ x, .some x = HsTerm.neutral_form t ∧ test x.fst
+
+inductive ValidHsCtorType : Ctx HsTerm -> HsTerm -> Prop where
+| refl :
+  HsValidHeadVariable R Γ.is_datatype ->
+  ValidHsCtorType Γ R
+| arrow :
+  ValidHsCtorType (.empty::Γ) B ->
+  ValidHsCtorType Γ (A → B)
+| farrow :
+  ValidHsCtorType (.empty::Γ) B ->
+  ValidHsCtorType Γ (A ⇒ B)
+| all :
+  ValidHsCtorType (.kind A::Γ) B ->
+  ValidHsCtorType Γ (`∀{A} B)
+
+
+inductive ValidHsInstType : Ctx HsTerm -> HsTerm -> Prop where
+| refl :
+  HsValidHeadVariable R Γ.is_opent ->
+  ValidHsInstType Γ R
+| arrow :
+  ValidHsInstType (.empty::Γ) B ->
+  ValidHsInstType Γ (A → B)
+| farrow :
+  ValidHsInstType (.empty::Γ) B ->
+  ValidHsInstType Γ (A ⇒ B)
+| all :
+  ValidHsInstType (.kind A::Γ) B ->
+  ValidHsInstType Γ (`∀{A} B)
+
+inductive StableHsTypeMatch : Ctx HsTerm -> HsTerm -> HsTerm -> Prop where
+| refl :
+  HsValidHeadVariable R Γ.is_stable ->
+  StableHsTypeMatch Γ R R
+| arrow :
+  HsValidHeadVariable R (Ctx.is_stable Γ) ->
+  StableHsTypeMatch (.empty::Γ) B ([S]R) ->
+  StableHsTypeMatch Γ (A → B) R
+| farrow :
+  HsValidHeadVariable R (Ctx.is_stable Γ) ->
+  StableHsTypeMatch (.empty::Γ) B ([S]R) ->
+  StableHsTypeMatch Γ (A ⇒ B) R
+| all :
+  HsValidHeadVariable R (Ctx.is_stable Γ) ->
+  StableHsTypeMatch (.kind A::Γ) B ([S]R) ->
+  StableHsTypeMatch Γ (`∀{A} B) R
+
+inductive PrefixHsTypeMatch : Ctx HsTerm -> HsTerm -> HsTerm -> HsTerm -> Prop where
+| refl :
+  HsValidHeadVariable B Γ.is_stable ->
+  PrefixHsTypeMatch Γ B T T
+| arrow :
+  PrefixHsTypeMatch (.empty::Γ) B V ([S]T) ->
+  PrefixHsTypeMatch Γ (A → B) (A → V) T
+| all :
+  PrefixHsTypeMatch (.kind A::Γ) B V ([S]T) ->
+  PrefixHsTypeMatch Γ (`∀{A} B) (`∀{A} V) T
+
+
+@[simp]
+abbrev HsJudgmentArgs : JudgmentVariant -> Type
+| JudgmentVariant.wf => Unit
+| JudgmentVariant.prf => HsTerm × HsTerm
+
+
+inductive HsJudgment : (v : JudgmentVariant) -> Ctx HsTerm -> HsJudgmentArgs v -> Type where
+--------------------------------------------------------------------------------------
+---- Well-Formed Contexts and Declarations
+--------------------------------------------------------------------------------------
+| wfnil :  HsJudgment .wf [] ()
+| wfempty :
+  HsJudgment .wf Γ () ->
+  HsJudgment .wf (.empty::Γ) ()
+| wftype :
+  HsJudgment .prf Γ (A, `★) ->
+  HsJudgment .wf Γ () ->
+  HsJudgment .wf (.type A::Γ) ()
+| wfkind :
+  HsJudgment .prf Γ (A, `□) ->
+  HsJudgment .wf Γ () ->
+  HsJudgment .wf (.kind A::Γ) ()
+| wfdatatype :
+  HsJudgment .prf Γ (A, `□) ->
+  HsJudgment .wf Γ () ->
+  HsJudgment .wf (.datatype A::Γ) ()
+| wfctor :
+  HsJudgment .prf Γ (A, `★) ->
+  HsJudgment .wf Γ () ->
+  ValidHsCtorType Γ A ->
+  HsJudgment .wf (.ctor A::Γ) ()
+| wfopent :
+  HsJudgment .prf Γ (A, `□) ->
+  HsJudgment .wf Γ () ->
+  HsJudgment .wf (.opent A::Γ) ()
+| wfopenm :
+  HsJudgment .prf Γ (A, `★) ->
+  HsJudgment .wf Γ () ->
+  HsJudgment .wf (.openm A::Γ) ()
+| wfinsttype :
+  HsJudgment .prf Γ (A, `★) ->
+  HsJudgment .wf Γ () ->
+  ValidHsInstType Γ A ->
+  HsJudgment .wf (.insttype A::Γ) ()
+| wfinst :
+  .openm T = Γ d@ x ->
+  HsJudgment .prf Γ (t, T) ->
+  HsJudgment .wf Γ () ->
+  HsJudgment .wf (.inst `#x t::Γ) ()
+| wfterm :
+  HsJudgment .prf Γ (A, `★) ->
+  HsJudgment .prf Γ (t, A) ->
+  HsJudgment .wf Γ () ->
+  HsJudgment .wf (.term A t::Γ) ()
+
+-----------------------------------
+-- Implicits
+-----------------------------------
+| implicitArrI :
+  HsJudgment .prf Γ (π, `★) ->
+  HsJudgment .prf (.empty :: Γ) (t, τ) ->
+  HsJudgment .prf Γ (e, π) ->
+  HsJudgment .prf Γ (t, π ⇒ τ) -- F a => τ
+| implicitArrE :
+  HsJudgment .prf Γ (t, π ⇒ τ) -> -- F a => τ
+  HsJudgment .prf Γ (e, π) ->
+  HsJudgment .prf Γ (t, τ β[e])
+| implicitAllI :
+  HsJudgment .prf (.kind A :: Γ) (t, τ) ->
+  HsJudgment .prf Γ (A, `□) ->
+  HsJudgment .prf Γ (t, `∀{A} τ)
+| implicitAllE :
+  HsJudgment .prf Γ (t, `∀{A} τ) ->
+  HsJudgment .prf Γ (e, A) ->
+  HsJudgment .prf Γ (t, τ β[e])
+
+------------------------------------
+--- Terms
+------------------------------------
+| var :
+  HsJudgment .prf Γ (T, `★) ->
+  (Γ d@ x).get_type = .some T ->
+  HsJudgment .prf Γ (`#x, T)
+| lam :
+  HsJudgment .prf Γ (A, `★) ->
+  HsJudgment .prf Γ (A → B, `★) ->
+  HsJudgment .prf (.type A :: Γ) (t, B) ->
+  HsJudgment .prf Γ (`λ{A} t, A → B)
+| app :
+  HsJudgment .prf Γ (t1, A → B) ->
+  HsJudgment .prf Γ (t2, A) ->
+  B' = B β[A] ->
+  HsJudgment .prf Γ (t1 `• t2,  B')
+| hslet :
+  HsJudgment .prf Γ (t1,  A) ->
+  HsJudgment .prf (.term A t1 :: Γ) (t2, [S] B) ->
+  HsJudgment .prf Γ (.HsLet A t1 t2,  B)
+| hsIte :
+  HsJudgment .prf Γ (t1, A) ->
+  HsJudgment .prf Γ (t2, R) ->
+  HsJudgment .prf Γ (t3, B) ->
+  HsJudgment .prf Γ (t4, T) ->
+  HsJudgment .prf Γ (T, `★) ->
+  HsJudgment .prf Γ (R, `★) ->
+  StableHsTypeMatch Γ A R ->
+  PrefixHsTypeMatch Γ A B T ->
+  HsValidHeadVariable R Γ.is_datatype ->
+  HsValidHeadVariable t1 Γ.is_ctor ->
+  HsJudgment .prf Γ (.HsIte t1 t2 t3 t4,  T)
+
+notation:170 Γ:170 " ⊢s " t:170 " : " A:170 => HsJudgment JudgmentVariant.prf Γ (t, A)
+notation:170 "⊢s " Γ:170 => HsJudgment JudgmentVariant.wf Γ ()
+
+
+-- theorem hsJ_preserves_kinds : Γ ⊢s t : τ -> Γ ⊢s τ : ★ := by
+-- intro j; induction j;
+-- case _ => assumption
+-- case _ => apply Judgment.arrow; assumption; assumption
+-- case implicitArrE e h1 h2 h3 =>
+--   cases h3; case _ h3 =>
+--   have lem := beta_empty e h3; simp at lem; assumption;
+-- case implicitAllI h1 h2 =>
+--   apply Judgment.allt; assumption; assumption
+-- case implicitAllE h1 h2 =>
+--   cases h2; case _ h =>
+--   have lem := beta_kind h h1; simp at lem; assumption;
+-- case _ => assumption
+-- case _ A _ _ _ _ _ h1 h2 h3 =>
+--   cases h2; case _ h2 =>
+--   have lem := beta_empty A h2; simp at lem; rw [h1]; assumption
+-- case letterm j1 j2 h1 h2 =>
+--   sorry
+-- case _ h => assumption
