Hs/HsTerm.lean
@@ -1,0 +1,2 @@
+import Hs.HsTerm.Definition
+import Hs.HsTerm.Substitution
