Hs/HsTerm/Definition.lean
@@ -1,0 +1,170 @@
+import SystemFD.Ctx
+
+inductive HsCtor2Variant : Type where
+| arrowk -- a -k> b
+| appk   -- a `•k b
+| app    -- a `• b
+
+inductive HsBind2Variant : Type where
+| all   -- ∀[A] B
+| lam   -- `λ[A] B
+| arrow -- a → b
+| farrow -- a ⇒ b
+
+-- Surface syntax terms
+inductive HsTerm : Type where
+| HsType : HsTerm -- ★
+| HsKind : HsTerm -- "□"
+| HsVar : Nat -> HsTerm
+| HsCtor2 : HsCtor2Variant -> HsTerm -> HsTerm -> HsTerm
+| HsBind2 : HsBind2Variant -> HsTerm -> HsTerm -> HsTerm
+| HsLet : HsTerm -> HsTerm -> HsTerm -> HsTerm
+| HsIte : HsTerm -> HsTerm -> HsTerm -> HsTerm -> HsTerm
+
+protected def HsTerm.repr : (a : HsTerm) -> (p : Nat) -> Std.Format
+| HsType, _ => "`★"
+| HsKind, _ => "`□"
+| HsVar n , _ => "`#" ++ Nat.repr n
+| HsCtor2 .arrowk a b, p => (HsTerm.repr a p) ++ " `-k> " ++ (HsTerm.repr b p)
+| HsCtor2 .appk a b, p => (HsTerm.repr a p) ++ " `•k " ++ (HsTerm.repr b p)
+| HsCtor2 .app a b, p => (HsTerm.repr a p) ++ " `• " ++ (HsTerm.repr b p)
+| HsBind2 .lam t1 t2 , p => "`λ" ++ Std.Format.sbracket (HsTerm.repr t1 p) ++ HsTerm.repr t2 p
+| HsBind2 .all t1 t2 , p => "`∀" ++ Std.Format.sbracket (HsTerm.repr t1 p) ++ HsTerm.repr t2 p
+| HsBind2 .arrow t1 t2 , p => Repr.addAppParen ((HsTerm.repr t1 p) ++ " → " ++ HsTerm.repr t2 p) p
+| HsBind2 .farrow t1 t2 , p => Repr.addAppParen ((HsTerm.repr t1 p) ++ " ⇒ " ++ HsTerm.repr t2 p) p
+| HsLet t1 t2 t3 , p => "HsLet " ++ HsTerm.repr t2 p ++ " : " ++ HsTerm.repr t1 p ++";;" ++ Std.Format.line ++ HsTerm.repr t3 p
+| HsIte t1 t2 t3 t4, p =>
+  "HsIf" ++ HsTerm.repr t1 p ++ " ← " ++ HsTerm.repr t2 p ++
+  "then" ++ Std.Format.line ++ HsTerm.repr t3 p ++
+  "else" ++ Std.Format.line ++ HsTerm.repr t4 p
+
+instance HsTerm_repr : Repr HsTerm where
+  reprPrec a p := HsTerm.repr a p
+
+notation "`★" => HsTerm.HsType
+notation "`□" => HsTerm.HsKind
+infixl:15 " `• " => HsTerm.HsCtor2 HsCtor2Variant.app
+infixl:15 " `•k " => HsTerm.HsCtor2 HsCtor2Variant.appk
+notation:15  a " `-k> " b => HsTerm.HsCtor2 HsCtor2Variant.arrowk a b
+notation:15 "`λ{" a "}" b => HsTerm.HsBind2 HsBind2Variant.lam a b
+notation:15 "`∀{" a "}" b => HsTerm.HsBind2 HsBind2Variant.all a b
+notation:15  a " → " b => HsTerm.HsBind2 HsBind2Variant.arrow a b
+notation:15  a " ⇒ " b => HsTerm.HsBind2 HsBind2Variant.farrow a b
+prefix:max "`#" => HsTerm.HsVar
+notation:15 "HsIf " p " ← " s " then " i " else " e => HsTerm.HsIte p s i e
+
+namespace HsTerm
+ @[simp]
+ def size : HsTerm -> Nat
+ | HsType => 0
+ | HsKind => 0
+ | HsVar _ => 0
+ | HsCtor2 _ t1 t2 => size t1 + size t2 + 1
+ | HsBind2 _ t1 t2 => size t1 + size t2 + 1
+ | HsLet t1 t2 t3 => size t1 + size t2 + size t3 + 1
+ | HsIte _ t1 t2 t3 => size t1 + size t2 + size t3 + 1
+end HsTerm
+
+instance sizeOf_HsTerm : SizeOf HsTerm where
+  sizeOf := HsTerm.size
+
+namespace HsCtor2Variant
+  @[simp]
+  def beq : HsCtor2Variant -> HsCtor2Variant -> Bool
+  | arrowk, arrowk => true
+  | appk, appk => true
+  | app, app => true
+  | _, _ => false
+end HsCtor2Variant
+
+@[simp]
+instance instBEq_HsCtor2Variant : BEq HsCtor2Variant where
+  beq := HsCtor2Variant.beq
+
+instance instLawfulBEq_HsCtor2Variant : LawfulBEq HsCtor2Variant where
+  eq_of_beq := by
+    intro a b h; simp at h
+    cases a <;> cases b <;> simp at *
+  rfl := by
+    intro a; simp
+    cases a <;> simp
+
+namespace HsBind2Variant
+  @[simp]
+  def beq : HsBind2Variant -> HsBind2Variant -> Bool
+  | all, all => true
+  | lam, lam => true
+  | arrow, arrow => true
+  | farrow, farrow => true
+  | _, _ => false
+end HsBind2Variant
+
+@[simp]
+instance instBEq_HsBind2Variant : BEq HsBind2Variant where
+  beq := HsBind2Variant.beq
+
+instance instLawfulBEq_HsBind2Variant : LawfulBEq HsBind2Variant where
+  eq_of_beq := by
+    intro a b h; simp at h
+    cases a <;> cases b <;> simp at *
+  rfl := by
+    intro a; simp
+    cases a <;> simp
+
+namespace HsTerm
+  @[simp]
+  def beq : HsTerm -> HsTerm -> Bool
+  | HsKind, HsKind => true
+  | HsType, HsType => true
+  | HsVar x, HsVar y => x == y
+  | HsIte x1 x2 x3 x4, HsIte y1 y2 y3 y4 =>
+    beq x1 y1 && beq x2 y2 && beq x3 y3 && beq x4 y4
+  | HsLet x1 x2 x3, HsLet y1 y2 y3 =>
+    beq x1 y1 && beq x2 y2 && beq x3 y3
+  | HsCtor2 v1 x1 x2, HsCtor2 v2 y1 y2 =>
+    v1 == v2 && beq x1 y1 && beq x2 y2
+  | HsBind2 v1 x1 x2, HsBind2 v2 y1 y2 =>
+    v1 == v2 && beq x1 y1 && beq x2 y2
+  | _, _ => false
+
+  theorem eq_of_beq : HsTerm.beq a b = true -> a = b := by
+  intro h
+  induction a generalizing b
+  case HsCtor2 v1 x1 x2 ih1 ih2 =>
+    cases b
+    case HsCtor2 v2 y1 y2 =>
+      have lem := @LawfulBEq.eq_of_beq HsCtor2Variant _ _ v1 v2
+      simp at *; replace lem := lem h.1.1
+      rw [lem, ih1 h.1.2, ih2 h.2]; simp
+    all_goals (simp at *)
+  case HsBind2 v1 x1 x2 ih1 ih2 =>
+    cases b
+    case HsBind2 v2 y1 y2 =>
+      have lem := @LawfulBEq.eq_of_beq HsBind2Variant _ _ v1 v2
+      simp at *; replace lem := lem h.1.1
+      rw [lem, ih1 h.1.2, ih2 h.2]; simp
+    all_goals (simp at *)
+  any_goals (cases b <;> simp at *)
+
+  case _ => simp [*]
+
+  case _ ih1 ih2 ih3 _ _ _ =>
+    rw [ih1 h.1.1, ih2 h.1.2]
+    rw [ih3 h.2]; simp
+
+  case _ ih1 ih2 ih3 ih4 _ _ _ _ =>
+    rw [ih1 h.1.1.1, ih2 h.1.1.2]
+    rw [ih3 h.1.2, ih4 h.2]; simp
+
+  theorem rfl : HsTerm.beq a a = true := by
+  induction a <;> simp at * <;> simp [*]
+
+end HsTerm
+
+@[simp]
+instance instBEq_HsTerm : BEq HsTerm where
+  beq := HsTerm.beq
+
+instance instLawfulBEq_HsTerm : LawfulBEq HsTerm where
+  eq_of_beq := HsTerm.eq_of_beq
+  rfl := HsTerm.rfl
