Hs/HsTerm/Substitution.lean
@@ -1,0 +1,290 @@
+import SystemFD.Substitution
+import SystemFD.Ctx
+import Hs.HsTerm.Definition
+import SystemFD.Util
+
+
+inductive HsSpineVariant where
+| term | kind
+deriving Repr
+
+namespace HsSpineVariant
+  @[simp]
+  def beq : HsSpineVariant -> HsSpineVariant -> Bool
+  | HsSpineVariant.term, HsSpineVariant.term => true
+  | .kind, .kind => true
+  | _, _ => false
+end HsSpineVariant
+
+@[simp]
+instance instBEq_HsSpineVariant : BEq HsSpineVariant where
+  beq := HsSpineVariant.beq
+
+instance instLawfulBEq_HsSpineVariant : LawfulBEq HsSpineVariant where
+  eq_of_beq := by
+    intro a b h; simp at h
+    cases a <;> cases b <;> simp at *
+  rfl := by
+    intro a; simp
+    cases a <;> simp
+
+
+namespace HsTerm
+  @[simp]
+  def neutral_form : HsTerm -> Option (Nat × List (HsSpineVariant × HsTerm))
+  | .HsVar x => .some (x, [])
+  | .HsCtor2 .app f a => do
+    let (x, sp) <- neutral_form f
+    .some (x, sp ++ [(HsSpineVariant.term, a)])
+  | .HsCtor2 .appk f a => do
+    let (x, sp) <- neutral_form f
+    .some (x, sp ++ [(.kind, a)])
+  | _ => .none
+
+  @[simp]
+  def apply_spine : HsTerm -> List (HsSpineVariant × HsTerm) -> HsTerm
+  | t, [] => t
+  | t, .cons (.term, h) tl => apply_spine (t `• h) tl
+  | t, .cons (.kind, h) tl => apply_spine (t `•k h) tl
+
+  theorem apply_spine_peel_term :
+    apply_spine f (sp ++ [(.term, a)]) = (apply_spine f sp `• a)
+  := by
+  induction f, sp using apply_spine.induct <;> simp
+  all_goals (case _ ih => rw [ih])
+
+  theorem apply_spine_peel_kind :
+    apply_spine f (sp ++ [(.kind, a)]) = (apply_spine f sp `•k a)
+  := by
+  induction f, sp using apply_spine.induct <;> simp
+  all_goals (case _ ih => rw [ih])
+
+  theorem var_neutral_form : (HsVar n).neutral_form = .some (n, []) := by
+  unfold HsTerm.neutral_form; rfl
+
+  theorem neutral_form_app {f : HsTerm} :
+  f.neutral_form = .some (h, sp) ->
+  (f `• t).neutral_form = .some (h, sp ++ [(.term, t)]) := by
+  intros h; simp_all
+
+  theorem neutral_form_appk {f : HsTerm}:
+  f.neutral_form = .some (h, sp) ->
+  (f `•k t).neutral_form = .some (h, sp ++ [(.kind, t)])
+  := by intros h; simp_all
+
+  theorem unique_neutral_form : (HsTerm.neutral_form t = .some (n, sp))
+                            -> (HsTerm.neutral_form t = .some (n', sp')) -> (n = n' ∧ sp = sp') := by
+  intros tnf tnf';
+  induction t using HsTerm.neutral_form.induct;
+  any_goals (solve | simp_all)
+
+  theorem neutral_form_app_rev {f : HsTerm}:
+  (f `• t).neutral_form = .some (h, sp ++ [(.term, t)] ) ->
+  f.neutral_form = .some (h, sp) := by
+  intros h; simp_all;
+  case _ n =>
+  rw [Option.bind_eq_some] at h; cases h; case _ w h =>
+  simp at h; have h2 := h.2.1; have h3 := h.2.2;
+  subst h2; subst h3; simp_all;
+
+  theorem neutral_form_appk_rev_exists {f : HsTerm} :
+  (f `•k t).neutral_form = .some (h, sp) ->
+  ∃ sp', f.neutral_form = .some (h, sp') ∧ sp = sp' ++ [(.kind , t)] := by
+  intros h; simp_all;
+  case _ n =>
+  rw [Option.bind_eq_some] at h; cases h; case _ w h =>
+  simp at h; have h2 := h.2.1; have h3 := h.2.2;
+  subst h2; subst h3; simp_all;
+
+  theorem neutral_form_bind2 : (HsTerm.HsBind2 a1 a2 a3).neutral_form = .none := by
+  unfold HsTerm.neutral_form; rfl
+
+  theorem neutral_form_ite : (HsTerm.HsIte p s i e).neutral_form = .none := by
+  unfold HsTerm.neutral_form; rfl
+
+  theorem neutral_form_letterm : (HsTerm.HsLet a1 a2 a3).neutral_form = .none := by
+  unfold HsTerm.neutral_form; rfl
+
+  theorem apply_spine_compose :
+    HsTerm.apply_spine t (t1 ++ t2) = HsTerm.apply_spine (HsTerm.apply_spine t t1) t2
+  := by
+  induction t, t1 using HsTerm.apply_spine.induct generalizing t2
+  case _ => simp
+  all_goals (case _ ih => simp; rw [ih])
+
+  theorem neutral_form_law :
+    .some (x, sp) = HsTerm.neutral_form t ->
+    HsTerm.apply_spine `#x sp = t
+  := by
+  intro h; induction t using neutral_form.induct generalizing x sp
+  case _ =>
+    simp at h; cases h; case _ h1 h2 =>
+      subst h1; subst h2; simp
+  case _ ih =>
+    simp at h; replace h := Eq.symm h
+    rw [Option.bind_eq_some] at h; simp at h
+    cases h; case _ a h =>
+    cases h; case _ b h =>
+    cases h; case _ h1 h2 =>
+    cases h2; case _ h2 h3 =>
+      subst h2; subst h3
+      replace ih := ih (Eq.symm h1)
+      rw [apply_spine_peel_term, ih]
+  case _ ih =>
+    simp at h; replace h := Eq.symm h
+    rw [Option.bind_eq_some] at h; simp at h
+    cases h; case _ a h =>
+    cases h; case _ b h =>
+    cases h; case _ h1 h2 =>
+    cases h2; case _ h2 h3 =>
+      subst h2; subst h3
+      replace ih := ih (Eq.symm h1)
+      rw [apply_spine_peel_kind, ih]
+  case _ h1 h2 h3 h4 => simp at h
+
+
+  @[simp]
+  def smap (lf : Subst.Lift HsTerm) (f : Nat -> Subst.Action HsTerm) : HsTerm -> HsTerm
+  | HsVar x =>
+    match f x with
+    | .re y => HsVar y
+    | .su t => t
+  | HsKind => HsKind
+  | HsType => HsType
+  | HsCtor2 v t1 t2 => HsCtor2 v (smap lf f t1) (smap lf f t2)
+  | HsBind2 v t1 t2 => HsBind2 v (smap lf f t1) (smap lf (lf f) t2)
+  | HsIte t1 t2 t3 t4 => .HsIte (smap lf f t1) (smap lf f t2) (smap lf f t3) (smap lf f t4)
+  | HsLet t1 t2 t3 => HsLet (smap lf f t1) (smap lf f t2) (smap lf (lf f) t3)
+end HsTerm
+
+@[simp]
+instance substType_HsTerm : SubstitutionType HsTerm where
+  smap := HsTerm.smap
+
+namespace HsTerm
+  @[simp↓]
+  theorem subst_var : [σ](HsTerm.HsVar x) = match σ x with | .re y => .HsVar y | .su t => t := by
+  unfold Subst.apply; simp
+
+  @[simp] -- 0[s.σ ] = s
+  theorem subst_HsVar_replace
+    : [.su s :: σ](HsVar 0) = s
+  := by simp
+
+  @[simp] -- 0[s.σ ] = s
+  theorem subst_HsVar_rename
+    : [.re k :: σ](HsVar 0) = HsVar k
+  := by simp
+
+  @[simp]
+  theorem subst_HsKind : [σ]HsKind = HsKind := by unfold Subst.apply; simp
+
+  @[simp]
+  theorem subst_const : [σ]HsType = HsType := by unfold Subst.apply; simp
+
+  @[simp]
+  theorem subst_HsIte : [σ]HsIte t1 t2 t3 t4 = HsIte ([σ]t1) ([σ]t2) ([σ]t3) ([σ]t4) := by unfold Subst.apply; simp
+
+  @[simp]
+  theorem subst_HsCtor2 : [σ]HsCtor2 v t1 t2 = HsCtor2 v ([σ]t1) ([σ]t2) := by unfold Subst.apply; simp
+
+  @[simp]
+  theorem subst_HsBind2 : [σ]HsBind2 v t1 t2 = HsBind2 v ([σ]t1) ([^σ]t2) := by unfold Subst.apply; simp
+
+  @[simp]
+  theorem subst_letterm: [σ]HsLet t1 t2 t3 = HsLet ([σ]t1) ([σ]t2) ([^σ]t3) := by unfold Subst.apply; simp
+
+
+  theorem apply_id {t : HsTerm} : [I]t = t := by
+  have lem1 : ^I = @I HsTerm := by
+    funext; case _ x =>
+    cases x; all_goals (unfold Subst.lift; unfold I; simp)
+  induction t
+  all_goals (simp at * <;> try simp [*])
+
+  theorem apply_stable {r : Ren} {σ : Subst HsTerm}
+    : r.to = σ -> Ren.apply r = Subst.apply σ
+  := by
+  intro h; funext; case _ x =>
+    unfold Ren.apply; simp at *
+    unfold Ren.to; simp
+    induction x generalizing r σ <;> simp at *
+    case _ x => rw [<-h]; unfold Ren.to; simp
+    all_goals simp [*]
+    all_goals (
+      rw [Subst.lift_lemma, <-h]
+      unfold Ren.fro; simp
+    )
+
+  theorem apply_compose {s : HsTerm} {σ τ : Subst HsTerm} : [τ][σ]s = [τ ⊙ σ]s := by
+  solve_compose HsTerm, apply_stable, s, σ, τ
+
+  @[simp]
+  def to_telescope : HsTerm -> Ctx HsTerm × HsTerm
+  | HsBind2 .arrow A B =>
+    let (Γ, r) := to_telescope B
+    (.type A::Γ, r)
+  | `∀{A} B =>
+    let (Γ, r) := to_telescope B
+    (.kind A::Γ, r)
+  | t => ([], t)
+
+  @[simp]
+  def from_telescope_rev : Ctx HsTerm -> HsTerm -> HsTerm
+  | [], t => t
+  | .cons (.type A) Γ, t => from_telescope_rev Γ (.HsBind2 .arrow A t)
+  | .cons (.kind A) Γ, t => from_telescope_rev Γ (`∀{A} t)
+  | .cons _ Γ, t => from_telescope_rev Γ t
+
+  @[simp]
+  def from_telescope (Γ : Ctx HsTerm) (t : HsTerm) : HsTerm :=
+    from_telescope_rev Γ.reverse t
+
+  theorem telescope_neutral_form_lemma {t : HsTerm} :
+    t.neutral_form = .some (x, xs) ->
+    t.to_telescope = ([], t) := by
+    induction t;
+    any_goals (solve | simp_all)
+
+  theorem unique_telescope {t : HsTerm} :
+    t.to_telescope = (x, xs) ->
+    t.to_telescope = (x', xs') ->
+    x = x' ∧ xs = xs' :=  by
+    intros h1 h2; rw [h1] at h2; simp at h2; assumption;
+
+end HsTerm
+
+instance substTypeLaws_HsTerm : SubstitutionTypeLaws HsTerm where
+  apply_id := HsTerm.apply_id
+  apply_compose := HsTerm.apply_compose
+  apply_stable := HsTerm.apply_stable
+
+  @[simp]
+  theorem hs_term_size_of_subst_rename {t : HsTerm} (r : Ren)
+    : HsTerm.size ([r.to]t) = HsTerm.size t
+  := by
+  have lem (r : Ren) :
+    .re 0::((@S HsTerm) ⊙ r.to) = (Subst.size_of_subst_rename_renamer r).to
+  := by
+    unfold Ren.to; simp
+    funext; case _ x =>
+      cases x <;> simp
+      case _ n => unfold Subst.compose; simp
+  induction t generalizing r <;> simp [*]
+  case _ x => unfold Ren.to; simp
+
+  theorem hs_term_right_shifting_size_no_change {s : HsTerm} : s.size = ([S' k]s).size := by
+  have lem := @hs_term_size_of_subst_rename s (fun n => n + k);
+  unfold S'; rw [<-lem]; rfl
+
+  theorem hs_term_right_shifting_size_no_change1 {s : HsTerm} : s.size = ([S]s).size := by
+  have lem := @hs_term_right_shifting_size_no_change 1 s;
+  unfold S; unfold S' at lem; assumption
+
+  theorem hs_term_left_shifting_size_no_change {s : HsTerm} : s.size = ([P' k]s).size := by
+  have lem := @hs_term_size_of_subst_rename s (fun n => n - k);
+  unfold P'; rw [<-lem]; rfl
+
+  theorem hs_term_left_shifting_size_no_change1 {s : HsTerm} : s.size = ([P]s).size := by
+  have lem := @hs_term_left_shifting_size_no_change 1 s;
+  unfold P; unfold P' at lem; assumption
