lakefile.lean
@@ -3,11 +3,13 @@ open Lake DSL
 
 require "leanprover-community" / "mathlib" @ git "v4.18.0-rc1"
 
-package SystemFD where
+package SystemFD
   -- add package configuration options here
 
-lean_lib SystemFD where
+lean_lib SystemFD
   -- add library configuration options here
+lean_lib Hs
+
 
 @[default_target]
 lean_exe systemfd where
